forward sim Cmajor to Cminor done

src/Cmajortominor.v
@@ -13,6 +13,10 @@ Require Import compcert.common.Smallstep.
 Require Import compcert.backend.Cminor.
 Require Import Cmajor.
 
+Require Import StructTact.StructTactics.
+Require Import StructTact.Util.
+
+
 Fixpoint transf_expr (e : Cmajor.expr) : Cminor.expr :=
   match e with
   | Evar id => Cminor.Evar id
@@ -55,14 +59,386 @@ Let ge := Genv.globalenv prog.
 Let tge := Genv.globalenv tprog.
 Hypothesis TRANSF : transf_prog prog = tprog.
 
-(* Proof in here *)
-(* TODO: prove this *)
+(* extensionally equal environments *)
+Definition env_lessdef (e1 e2: env) : Prop :=
+  forall id v1, e1!id = Some v1 -> exists v2, e2!id = Some v2 /\ Val.lessdef v1 v2.
+
+Inductive match_cont: Cmajor.cont -> Cminor.cont -> Prop :=
+  | match_cont_stop:
+      match_cont Cmajor.Kstop Cminor.Kstop
+  | match_cont_seq: forall s s' k k',
+      transf_stmt s = s' ->
+      match_cont k k' ->
+      match_cont (Cmajor.Kseq s k) (Cminor.Kseq s' k')
+  | match_cont_block: forall k k',
+      match_cont k k' ->
+      match_cont (Cmajor.Kblock k) (Cminor.Kblock k')
+  | match_cont_call: forall id f sp e k f' e' k',
+      transf_function f = f' ->
+      match_cont k k' ->
+      env_lessdef e e' ->
+      match_cont (Cmajor.Kcall id f sp e k) (Cminor.Kcall id f' sp e' k').
+
+Inductive match_states : Cmajor.state -> Cminor.state -> Prop :=
+  | match_state: forall f f' s k s' k' sp e m e' m'
+        (TF: transf_function f = f')
+        (TS: transf_stmt s = s')
+        (MC: match_cont k k')
+        (LD: env_lessdef e e')
+        (ME: Mem.extends m m'),
+      match_states
+        (Cmajor.State f s k sp e m)
+        (Cminor.State f' s' k' sp e' m')
+  | match_callstate: forall f f' args args' k k' m m'
+        (TF: transf_fundef f = f')
+        (MC: match_cont k k')
+        (LD: Val.lessdef_list args args')
+        (ME: Mem.extends m m'),
+      match_states
+        (Cmajor.Callstate f args k m)
+        (Cminor.Callstate f' args' k' m')
+  | match_returnstate: forall v v' k k' m m'
+        (MC: match_cont k k')
+        (LD: Val.lessdef v v')
+        (ME: Mem.extends m m'),
+      match_states
+        (Cmajor.Returnstate v k m)
+        (Cminor.Returnstate v' k' m').
+
+Remark call_cont_commut:
+  forall k k', match_cont k k' -> match_cont (Cmajor.call_cont k) (Cminor.call_cont k').
+Proof.
+  induction 1; simpl; auto. constructor. constructor; auto.
+Qed.
+
+Lemma is_call_cont_transf :
+  forall k k',
+    Cmajor.is_call_cont k ->
+    match_cont k k' ->
+    Cminor.is_call_cont k'.
+Proof.
+  intros. destruct k; simpl in *; try solve [inv H]; inv H0; eauto.
+Qed.
+
+Ltac invp pat :=
+  match goal with
+  | [ H : context[pat] |- _ ] => inversion H
+  end.
+
+Lemma eval_expr_transf :
+  forall a e m v,
+    Cmajor.eval_expr e m a v ->
+    forall tge sp e' m',
+      env_lessdef e e' ->
+      Mem.extends m m' ->
+      exists v',
+        Cminor.eval_expr tge sp e' m' (transf_expr a) v' /\ Val.lessdef v v'.
+Proof.
+  induction a; intros.
+  * inv H.
+    unfold env_lessdef in *.
+    apply H0 in H3. break_exists. break_and.
+    eexists.
+    split. econstructor.
+    eassumption. assumption.
+  * inv H. eapply IHa in H4; eauto.
+    break_exists. break_and.
+    instantiate (1 := sp) in H2.
+    instantiate (1 := tge0) in H2.
+    simpl.
+    eapply Mem.loadv_extends in H6; eauto.
+    break_exists; break_and. 
+    exists x0. split; eauto.
+    econstructor; eauto.
+Qed.
+
+Lemma eval_exprlist_transf :
+  forall a e m v,
+    Cmajor.eval_exprlist e m a v ->
+    forall tge sp e' m',
+      env_lessdef e e' ->
+      Mem.extends m m' ->
+      exists v',
+        Cminor.eval_exprlist tge sp e' m' (map transf_expr a) v' /\ Val.lessdef_list v v'.
+Proof.
+  induction a; intros.
+  inversion H. subst v. eexists; split; econstructor; eauto.
+  inversion H.
+  remember tprog. subst.
+  eapply IHa in H6; eauto.
+  repeat break_exists; repeat break_and.
+  eapply eval_expr_transf in H4; eauto.
+  repeat break_exists; repeat break_and.
+  eexists; split; try econstructor; eauto.
+Qed.  
+
+Lemma env_lessdef_set :
+  forall id v v' e e',
+    Val.lessdef v v' ->
+    env_lessdef e e' ->
+    env_lessdef (PTree.set id v e) (PTree.set id v' e').
+Proof.
+  intros.
+  unfold env_lessdef in *.
+  intros.
+  destruct (peq id id0); subst.
+  rewrite PTree.gss in *. eexists; split; eauto. congruence.
+  rewrite PTree.gso in * by congruence.
+  apply H0 in H1. break_exists; break_and.
+  eexists; split; eauto.
+Qed.
+
+Lemma find_funct_transf :
+  forall vf vf',
+    Val.lessdef vf vf' ->
+    forall fd,
+      Genv.find_funct ge vf = Some fd ->
+      Genv.find_funct tge vf' = Some (transf_fundef fd).
+Proof.
+  intros.
+  remember H0 as H1. clear HeqH1.
+  eapply Genv.find_funct_transf in H0; eauto.
+  instantiate (1 := transf_fundef) in H0.
+  inv H. unfold tge. assumption.
+  simpl in H1. congruence.
+Qed.
+
+Lemma find_funct_ptr_transf :
+  forall b f,
+    Genv.find_funct_ptr ge b = Some f ->
+    Genv.find_funct_ptr tge b = Some (transf_fundef f).
+Proof.
+  intros.
+  unfold tge. rewrite <- TRANSF.
+  eapply Genv.find_funct_ptr_transf; eauto.
+Qed.
+  
+Lemma funsig_transf :
+  forall fd,
+    Cminor.funsig (transf_fundef fd) = funsig fd.
+Proof.
+  intros. destruct fd; simpl; reflexivity.
+Qed.
+
+Lemma find_symbol_transf :
+  forall id,
+    Genv.find_symbol tge id = Genv.find_symbol ge id.
+Proof.
+  intros. unfold tge.
+  unfold ge. rewrite <- TRANSF.
+  apply Genv.find_symbol_transf.
+Qed.
+
+Lemma public_symbol_transf :
+  forall id,
+    Genv.public_symbol tge id = Genv.public_symbol ge id.
+Proof.
+  intros. unfold tge.
+  unfold ge. rewrite <- TRANSF.
+  apply Genv.public_symbol_transf.
+Qed.
+
+Lemma find_var_info_transf :
+  forall b,
+    Genv.find_var_info tge b = Genv.find_var_info ge b.
+Proof.
+  intros. unfold tge.
+  unfold ge. rewrite <- TRANSF.
+  apply Genv.find_var_info_transf.
+Qed.
+
+Lemma external_call_transf :
+  forall ef vargs m t vres m',
+    external_call ef ge vargs m t vres m' ->
+    forall m0 vargs0,
+      Val.lessdef_list vargs vargs0 ->
+      Mem.extends m m0 ->
+      exists vres0 m0',
+        external_call ef tge vargs0 m0 t vres0 m0' /\ Mem.extends m' m0' /\ Val.lessdef vres vres0.
+Proof.
+  intros.
+  eapply external_call_mem_extends in H1; eauto.
+  repeat break_exists; repeat break_and.
+  exists x. exists x0.
+  split.
+  eapply external_call_symbols_preserved; eauto.
+  eapply find_symbol_transf.
+  eapply public_symbol_transf.
+  eapply find_var_info_transf.
+  split; assumption.
+Qed.
+
+Lemma match_call_cont :
+  forall k k',
+    match_cont k k' ->
+    match_cont (call_cont k) (Cminor.call_cont k').
+Proof.
+  induction 1; intros; simpl; try econstructor; eauto.
+Qed.
+
+Lemma env_lessdef_set_locals :
+  forall e e',
+    env_lessdef e e' ->
+    forall l,
+      env_lessdef (set_locals l e) (Cminor.set_locals l e').
+Proof.
+  induction l; intros.
+  simpl. assumption.
+  simpl. eapply env_lessdef_set; eauto.
+Qed.
+
+Lemma env_lessdef_set_params :
+  forall ids vs vs',
+    Val.lessdef_list vs vs' ->
+    env_lessdef (set_params vs ids) (Cminor.set_params vs' ids).
+Proof.
+  induction ids; intros.
+  simpl. unfold env_lessdef. intros. rewrite PTree.gempty in H0. congruence.
+  inversion H. remember tprog. subst. simpl. eapply env_lessdef_set; eauto.
+  simpl. eapply env_lessdef_set; eauto.
+Qed.
+
+Lemma single_step_correct:
+  forall S1 t S2, Cmajor.step ge S1 t S2 ->
+  forall T1, match_states S1 T1 ->
+   (exists T2, Cminor.step tge T1 t T2 /\ match_states S2 T2).
+Proof.
+  induction 1; intros; invp match_states;
+    try solve [simpl; inv MC; eexists; split; try econstructor; eauto];
+    remember tprog; subst.
+  * (* return *)
+    eapply Mem.free_parallel_extends in ME; eauto.
+    break_exists. break_and.
+    eexists; split; try econstructor; eauto.
+    eapply is_call_cont_transf; eauto.
+  * (* assign *)
+    eapply eval_expr_transf in H; eauto.
+    break_exists. break_and.
+    eexists; split; try econstructor; eauto.
+    eapply env_lessdef_set; eauto.
+  * (* store *)
+    eapply eval_expr_transf in H; eauto.
+    eapply eval_expr_transf in H0; eauto.
+    repeat break_exists; repeat break_and.
+    eapply Mem.storev_extends in ME; eauto.
+    repeat break_exists; repeat break_and.
+    eexists; split; try econstructor; eauto.
+  * (* call *)
+    eapply eval_expr_transf in H; eauto.
+    eapply eval_exprlist_transf in H0; eauto.
+    repeat break_exists; repeat break_and.
+    eexists; split; try econstructor; eauto; simpl.
+    eapply find_funct_transf; eauto.
+    eapply funsig_transf; eauto.
+    econstructor; eauto.
+  * (* builtin *)
+    eapply eval_exprlist_transf in H; eauto.
+    break_exists; break_and.
+    eapply external_call_transf in H0; eauto.
+    break_exists; break_and.
+    eexists; split; try econstructor; eauto; simpl.
+    destruct optid. simpl. eapply env_lessdef_set; eauto.
+    simpl. assumption.
+  * (* seq *)
+    simpl.
+    eexists; split; try econstructor; eauto.
+    econstructor; eauto.
+  * (* switch *)
+    simpl.
+    eapply eval_expr_transf in H; eauto.
+    break_exists; break_and.
+    eexists; split; try econstructor; eauto; simpl; eauto.
+    inv H0; inv H2; econstructor; eauto.
+  * (* return *)
+    simpl.
+    eapply Mem.free_parallel_extends in H; eauto.
+    break_exists; break_and.
+    eexists; split; try econstructor; eauto; simpl; eauto.
+    eapply match_call_cont; eauto.
+  * (* return *)
+    eapply eval_expr_transf in H; eauto.
+    eapply Mem.free_parallel_extends in H0; eauto.
+    repeat (break_exists; break_and).
+    eexists; split; try econstructor; eauto; simpl; eauto.
+    eapply match_call_cont; eauto.
+  * (* call internal *)
+    eapply Mem.alloc_extends in H; eauto.
+    break_exists. break_and.
+    eexists; split; try econstructor; eauto; simpl; eauto.
+    eapply env_lessdef_set_locals.
+    eapply env_lessdef_set_params; eauto.
+    omega.
+    simpl. omega.
+  * (* call external *)
+    eapply external_call_transf in H; eauto.
+    repeat break_exists; repeat break_and.
+    eexists; split; try econstructor; eauto; simpl; eauto.
+  * (* return *)
+    inversion MC. remember tprog. subst.
+    eexists; split; try econstructor; eauto; simpl; eauto.
+    destruct optid. simpl. eapply env_lessdef_set; eauto.
+    simpl. assumption.
+Qed.    
+
+Lemma init_mem_transf :
+  forall m,
+    Genv.init_mem prog = Some m ->
+    exists m',
+      Genv.init_mem tprog = Some m' /\ Mem.extends m m'.
+Proof.
+  intros.
+  eapply Genv.init_mem_transf in H.
+  unfold transf_prog in TRANSF. rewrite TRANSF in H.
+  exists m. split; eauto.
+  eapply Mem.extends_refl.
+Qed.
+
+Lemma match_final_state :
+ forall (s1 : Smallstep.state (semantics prog))
+        (s2 : Smallstep.state (Cminor.semantics tprog)) (r : int),
+   match_states s1 s2 ->
+   Smallstep.final_state (semantics prog) s1 r ->
+   Smallstep.final_state (Cminor.semantics tprog) s2 r.
+Proof.
+  intros.
+  inv H0. inv H.
+  inv LD.
+  inv MC.
+  econstructor; eauto.
+Qed.
+
+Lemma initial_states_match :
+  forall s1 : Smallstep.state (semantics prog),
+    Smallstep.initial_state (semantics prog) s1 ->
+    exists s2 : Smallstep.state (Cminor.semantics tprog),
+      Smallstep.initial_state (Cminor.semantics tprog) s2 /\ match_states s1 s2.
+Proof.
+  intros. 
+  inversion H.
+  eapply init_mem_transf in H0; try reflexivity.
+  break_exists; break_and.
+  eexists; split; econstructor; eauto;
+    simpl; try solve [econstructor; eauto].
+  erewrite find_symbol_transf; eauto.
+  rewrite <- TRANSF. simpl. eauto.
+  eapply find_funct_ptr_transf; eauto.
+  erewrite funsig_transf; eauto.  
+Qed.  
 
 End PRESERVATION.
 
 Theorem transf_program_correct:
   forall prog tprog,
-  forward_simulation (Cmajor.semantics prog) (Cminor.semantics tprog).
+    transf_prog prog = tprog ->
+    forward_simulation (Cmajor.semantics prog) (Cminor.semantics tprog).
 Proof.
+  intros.
+  eapply forward_simulation_step with (match_states := match_states).
+  eapply public_symbol_transf; eauto.
+  eapply initial_states_match; eauto.
+  eapply match_final_state; eauto.
+  eapply single_step_correct; eauto.
+Qed.
 
-Admitted.
+
+
